DynamoDbEncryption/dafny/DynamoDbItemEncryptor/src/Index.dfy
@@ -10,6 +10,7 @@ module
 {
   import opened DynamoDbItemEncryptorUtil
   import StructuredEncryption
+  import StructuredEncryptionHeader
   import CSE = AwsCryptographyDbEncryptionSdkStructuredEncryptionTypes
   import DDBE = AwsCryptographyDbEncryptionSdkDynamoDbTypes
   import MaterialProviders
@@ -37,31 +38,38 @@ module
     )
   }
 
-  // because an inline "!(ReservedPrefix <= attr)" is too hard for Dafny
   predicate method UnreservedPrefix(attr : string)
   {
-    !(ReservedPrefix <= attr)
+    && !(ReservedPrefix <= attr)
+    && !(SE.ReservedCryptoContextPrefixString <= attr)
   }
 
   predicate method IsVersion2Schema(actions : DDBE.AttributeActions)
   {
     exists x <- actions :: actions[x] == CSE.CONTEXT_AND_SIGN
   }
-  function method VersionFromActions(actions : DDBE.AttributeActions) : Operations.Version
+  function method VersionFromActions(actions : DDBE.AttributeActions) : StructuredEncryptionHeader.Version
   {
     if IsVersion2Schema(actions) then
       2
     else
       1
   }
-  function method KeyActionFromSchema(actions : DDBE.AttributeActions) : CSE.CryptoAction
+  function method KeyActionFromVersion(version : StructuredEncryptionHeader.Version) : CSE.CryptoAction
   {
-    if IsVersion2Schema(actions) then
+    if version == 2 then
       CSE.CONTEXT_AND_SIGN
     else
       CSE.SIGN_ONLY
-
   }
+  function method KeyActionStringFromVersion(version : StructuredEncryptionHeader.Version) : string
+  {
+    if version == 2 then
+      "CONTEXT_AND_SIGN"
+    else
+      "SIGN_ONLY"
+  }
+
 
   method {:vcs_split_on_every_assert} DynamoDbItemEncryptor(config: DynamoDbItemEncryptorConfig)
     returns (res: Result<IDynamoDbItemEncryptorClient, Error>)
@@ -82,10 +90,10 @@ module
       //# MUST be configured to the partition attribute and, if present, sort attribute.
       && rconfig.version == VersionFromActions(config.attributeActionsOnEncrypt)
       && config.partitionKeyName in config.attributeActionsOnEncrypt
-      && config.attributeActionsOnEncrypt[config.partitionKeyName] == KeyActionFromSchema(config.attributeActionsOnEncrypt)
+      && config.attributeActionsOnEncrypt[config.partitionKeyName] == KeyActionFromVersion(rconfig.version)
       && (config.sortKeyName.Some? ==>
           && config.sortKeyName.value in config.attributeActionsOnEncrypt
-          && config.attributeActionsOnEncrypt[config.sortKeyName.value] == KeyActionFromSchema(config.attributeActionsOnEncrypt))
+          && config.attributeActionsOnEncrypt[config.sortKeyName.value] == KeyActionFromVersion(rconfig.version))
 
     //= specification/dynamodb-encryption-client/ddb-table-encryption-config.md#plaintext-policy
     //# If not specified, encryption and decryption MUST behave according to `FORBID_PLAINTEXT_WRITE_FORBID_PLAINTEXT_READ`.
@@ -103,19 +111,20 @@ module
       message := "Must provide either a keyring or a CMM"
     ));
     var version := VersionFromActions(config.attributeActionsOnEncrypt);
-    var keyAction := KeyActionFromSchema(config.attributeActionsOnEncrypt);
+    var keyAction := KeyActionFromVersion(version);
+    var keyActionStr := KeyActionStringFromVersion(version);
     :- Need(
         && config.partitionKeyName in config.attributeActionsOnEncrypt
         && config.attributeActionsOnEncrypt[config.partitionKeyName] == keyAction,
       DynamoDbItemEncryptorException(
-        message := "Partition key attribute action MUST be SIGN_ONLY" // FIXME
+        message := "Partition key attribute action MUST be " + keyActionStr
       ));
     :- Need(
       (config.sortKeyName.Some? ==>
         && config.sortKeyName.value in config.attributeActionsOnEncrypt
         && config.attributeActionsOnEncrypt[config.sortKeyName.value] == keyAction),
       DynamoDbItemEncryptorException(
-        message := "Sort key attribute action MUST be SIGN_ONLY" // FIXME
+        message := "Sort key attribute action MUST be " + keyActionStr
       ));
 
     // We happen to order these values, but this ordering MUST NOT be relied upon.
